rocq/demo/CoRecursiveFunctionReificationDemo.v
@@ -1,0 +1,127 @@
+From impboot.functional Require Import FunSyntax FunValues FunSemantics.
+From impboot.imperative Require Import ImpSyntax Printing.
+From impboot.automation Require Import Ltac2Utils UnfoldFix RelCompiler RelCompilerCommons AutomationLemmas.
+From impboot Require Import fp2imp.FpToImpCodegen.
+From impboot Require Import assembly.ASMToString.
+From impboot Require Import parsing.Parser.
+From Stdlib Require Import List Bool NArith ZArith String Lia.
+From coqutil.Word Require Import Interface Properties.
+Import ListNotations.
+From Stdlib Require Import Derive.
+From Ltac2 Require Import Ltac2.
+From impboot.demo Require Import DemoUtils.
+
+CoInductive colist (A: Type): Type :=
+| conil: colist A
+| cocons: A -> colist A -> colist A.
+
+CoFixpoint encode_colist {A: Type} (l: colist A): FunValues.Value :=
+  match colist with
+  | conil _ => FunValues.Num 0
+  | cocons _ h t => FunValues.Pair (FunValues.Num 1) (FunValues.[h; encode_colist t])
+  end.
+
+(*  *)
+
+Fixpoint len (l: list nat): nat :=
+  match l with
+  | nil => 0%nat
+  | _ :: l1 => 1 + len l1
+  end.
+
+Theorem len_equation: ltac:(with_strategy opaque [Nat.add] ltac2:(unfold_fix_type '@len)).
+Proof. unfold_fix_proof '@len. Qed.
+
+Print len.
+
+Derive len_prog
+  in ltac2:(relcompile_tpe 'len_prog 'len [])
+  as len_prog_proof.
+Proof.
+  relcompile_setup ().
+  revert l. ltac1:(fix IH 1); intros.
+  eapply trans_app.
+  3: eauto. 2: reflexivity.
+
+  rewrite len_equation.
+  eapply auto_list_case with (n1 := "h") (n2 := "t").
+  3: ltac1:(shelve).
+  1: eapply trans_Var; unfold make_env; eauto with fenvDb.
+  destruct l.
+  1: eapply auto_nat_const.
+  eapply auto_nat_add.
+  1: eapply auto_nat_const.
+  eapply trans_Call; eauto.
+  eapply trans_Var.
+  unfold make_env; eauto with fenvDb.
+  Unshelve.
+  all: crush_side_conditions (); unfold name_enc in *; simpl in *; ltac1:(lia).
+Qed.
+Print len_prog.
+
+(* all: relcompile_start ().
+  all: relcompile_step ().
+  all: relcompile_step ().
+  all: relcompile_step ().
+  all: relcompile_step ().
+  Unshelve.
+  all: crush_side_conditions (); unfold name_enc in *; simpl in *; ltac1:(lia). *)
+
+
+
+
+
+
+
+
+
+
+
+
+
+
+
+
+
+
+
+
+
+
+
+
+
+(* Fixpoint even (n: nat): bool :=
+  match n with
+  | 0%nat => true
+  | S n => negb (odd n)
+  end
+with odd (n: nat): bool :=
+  match n with
+  | 0%nat => false
+  | S n => negb (even n)
+  end.
+
+Theorem even_equation: ltac2:(unfold_fix_type '@even).
+Proof. unfold_fix_proof '@even. Qed.
+
+Theorem odd_equation: ltac2:(unfold_fix_type '@odd).
+Proof. unfold_fix_proof '@odd. Qed.
+
+Ltac2 Set relcompile_one_step := false.
+
+Derive even_prog
+  in ltac2:(relcompile_tpe 'even_prog 'even ['odd])
+  as even_prog_proof.
+Proof.
+  time relcompile.
+Qed.
+Print even_prog.
+
+Derive odd_prog
+  in ltac2:(relcompile_tpe 'odd_prog 'odd ['even])
+  as odd_prog_proof.
+Proof.
+  time relcompile.
+Qed.
+Print odd_prog. *)
